{
 "cells": [
  {
   "cell_type": "markdown",
   "id": "0de8a3f8",
   "metadata": {},
   "source": [
    "# **Linear Recurrence Relations: The Complete Guide**\n",
    "\n",
    "## **What Is This?**\n",
    "A **linear recurrence relation** is an equation that defines a sequence where each term is a **linear combination** of previous terms, plus possibly an extra function.\n",
    "\n",
    "**Example you'll recognize:**\n",
    "- **Fibonacci:** \\(F_n = F_{n-1} + F_{n-2}\\) (each term = sum of previous two)\n",
    "- **Population growth:** \\(P_n = 1.05P_{n-1}\\) (5% growth each year)\n",
    "\n",
    "---\n",
    "\n",
    "## **Why Do We Care?**\n",
    "These appear **everywhere** in computer science:\n",
    "- **Algorithm analysis:** Divide-and-conquer algorithms (Merge Sort, Quick Sort)\n",
    "- **Dynamic programming:** Computing Fibonacci efficiently\n",
    "- **System modeling:** Queues, networks, finance\n",
    "- **Backtracking algorithms:** Counting paths, combinations\n",
    "\n",
    "---\n",
    "\n",
    "# **Quick Review of the Method**\n",
    "\n",
    "## **Standard Form:**\n",
    "\\[\n",
    "T(n) = a_1T(n-1) + a_2T(n-2) + \\cdots + a_kT(n-k) + f(n)\n",
    "\\]\n",
    "Where:\n",
    "- \\(T(n)\\) = term we want\n",
    "- \\(a_i\\) = constant coefficients\n",
    "- \\(f(n)\\) = \"forcing function\" (could be 0, constant, polynomial, exponential, etc.)\n",
    "\n",
    "---\n",
    "\n",
    "## **The 3-Step Solution Process:**\n",
    "\n",
    "\n",
    "\n",
    "**Solve for r:** Get roots \\(r_1, r_2, \\ldots, r_k\\)\n",
    "\n",
    "**Homogeneous solution:**\n",
    "- **Distinct real roots:** \\(T^{(h)}(n) = C_1 r_1^n + C_2 r_2^n + \\cdots + C_k r_k^n\\)\n",
    "- **Repeated root r (multiplicity m):** Include: \\(r^n, n r^n, n^2 r^n, \\ldots, n^{m-1} r^n\\)\n",
    "- **Complex roots:** \\(a \\pm bi\\) become \\(R^n(C_1 \\cos(n\\theta) + C_2 \\sin(n\\theta))\\)\n",
    "\n",
    "---\n",
    "\n",
    "### **Step 2: Find Particular Solution**\n",
    "For \\(f(n) \\neq 0\\), guess a form similar to \\(f(n)\\):\n",
    "\n",
    "| If \\(f(n)\\) is: | Guess \\(T^{(p)}(n)\\) is: |\n",
    "|-----------------|--------------------------|\n",
    "| **Constant c** | Constant A |\n",
    "| **Polynomial of degree d** | Polynomial of degree d |\n",
    "| **Exponential \\(c^n\\)** (c not a root) | \\(A \\cdot c^n\\) |\n",
    "| **Exponential \\(c^n\\)** (c is a root m times) | \\(A \\cdot n^m c^n\\) |\n",
    "| **sin/cos** | \\(A \\cos(\\omega n) + B \\sin(\\omega n)\\) |\n",
    "\n",
    "**Substitute guess into original recurrence** to solve for the unknown coefficients.\n",
    "\n",
    "---\n",
    "\n",
    "### **Step 3: Combine and Solve for Constants**\n",
    "\\[\n",
    "T(n) = T^{(h)}(n) + T^{(p)}(n)\n",
    "\\]\n",
    "Use **initial conditions** (like \\(T(0), T(1), \\ldots\\)) to find \\(C_1, C_2, \\ldots\\)\n",
    "\n",
    "---\n",
    "\n",
    "# **Examples from Easy to Hard**\n",
    "\n",
    "## **Example 1: Simple (Homogeneous)**\n",
    "\\[\n",
    "T(n) = 3T(n-1) - 2T(n-2), \\quad T(0)=0, T(1)=1\n",
    "\\]\n",
    "\n",
    "**Step 1:** Characteristic: \\(r^2 - 3r + 2 = 0\\)\n",
    "\\[\n",
    "(r-1)(r-2)=0 \\quad \\Rightarrow \\quad r=1, 2\n",
    "\\]\n",
    "\\[\n",
    "T^{(h)}(n) = C_1 \\cdot 1^n + C_2 \\cdot 2^n = C_1 + C_2 \\cdot 2^n\n",
    "\\]\n",
    "\n",
    "**Step 2:** \\(f(n)=0\\), so \\(T^{(p)}(n)=0\\)\n",
    "\n",
    "**Step 3:** Use initial:\n",
    "- \\(T(0)=0\\): \\(C_1 + C_2 = 0\\)\n",
    "- \\(T(1)=1\\): \\(C_1 + 2C_2 = 1\\)\n",
    "Solve: \\(C_1 = -1, C_2 = 1\\)\n",
    "\n",
    "\\[\n",
    "\\boxed{T(n) = 2^n - 1}\n",
    "\\]\n",
    "\n",
    "---\n",
    "\n",
    "## **Example 2: With Constant Term**\n",
    "\\[\n",
    "T(n) = 4T(n-1) - 3T(n-2) + 5, \\quad T(0)=1, T(1)=2\n",
    "\\]\n",
    "\n",
    "**Step 1:** Homogeneous: \\(T(n) - 4T(n-1) + 3T(n-2) = 0\\)\n",
    "Characteristic: \\(r^2 - 4r + 3 = 0\\)\n",
    "\\[\n",
    "(r-1)(r-3)=0 \\quad \\Rightarrow \\quad r=1, 3\n",
    "\\]\n",
    "\\[\n",
    "T^{(h)}(n) = C_1 \\cdot 1^n + C_2 \\cdot 3^n = C_1 + C_2 \\cdot 3^n\n",
    "\\]\n",
    "\n",
    "**Step 2:** \\(f(n)=5\\) (constant) → Guess \\(T^{(p)}(n) = A\\)\n",
    "Substitute: \\(A = 4A - 3A + 5\\) ⇒ \\(A = A + 5\\) ⇒ \\(0 = 5\\)? Wait, that's wrong!\n",
    "\n",
    "Actually: \\(A - 4A + 3A = 5\\) ⇒ \\(0 = 5\\) → **No solution!**\n",
    "\n",
    "Why? Because \\(r=1\\) is a root, so we need to **multiply by n**:\n",
    "Guess \\(T^{(p)}(n) = An\\) instead!\n",
    "\n",
    "Substitute \\(An\\):\n",
    "\\[\n",
    "An = 4A(n-1) - 3A(n-2) + 5\n",
    "\\]\n",
    "\\[\n",
    "An = 4An - 4A - 3An + 6A + 5\n",
    "\\]\n",
    "\\[\n",
    "An = An + 2A + 5\n",
    "\\]\n",
    "\\[\n",
    "0 = 2A + 5 \\quad \\Rightarrow \\quad A = -\\frac{5}{2}\n",
    "\\]\n",
    "So \\(T^{(p)}(n) = -\\frac{5}{2}n\\)\n",
    "\n",
    "**Step 3:** Combine:\n",
    "\\[\n",
    "T(n) = C_1 + C_2 \\cdot 3^n - \\frac{5}{2}n\n",
    "\\]\n",
    "Use initial:\n",
    "- \\(T(0)=1\\): \\(C_1 + C_2 = 1\\)\n",
    "- \\(T(1)=2\\): \\(C_1 + 3C_2 - \\frac{5}{2} = 2\\)\n",
    "Solve: \\(C_1 = \\frac{1}{4}, C_2 = \\frac{3}{4}\\)\n",
    "\n",
    "\\[\n",
    "\\boxed{T(n) = \\frac{1}{4} + \\frac{3}{4} \\cdot 3^n - \\frac{5}{2}n}\n",
    "\\]\n",
    "\n",
    "---\n",
    "\n",
    "## **Example 3: Your Type (Two Terms + f(n))**\n",
    "\\[\n",
    "T(n) = T(n-1) + 2T(n-2) + 2^n, \\quad T(0)=0, T(1)=1\n",
    "\\]\n",
    "\n",
    "**Step 1:** Characteristic: \\(r^2 - r - 2 = 0\\)\n",
    "\\[\n",
    "(r-2)(r+1)=0 \\quad \\Rightarrow \\quad r=2, -1\n",
    "\\]\n",
    "\\[\n",
    "T^{(h)}(n) = C_1 \\cdot 2^n + C_2 \\cdot (-1)^n\n",
    "\\]\n",
    "\n",
    "**Step 2:** \\(f(n)=2^n\\) → BUT \\(r=2\\) is already a root!\n",
    "So guess \\(T^{(p)}(n) = A n \\cdot 2^n\\) (multiply by n since 2 is a simple root)\n",
    "\n",
    "Substitute \\(A n 2^n\\):\n",
    "\\[\n",
    "A n 2^n = A (n-1) 2^{n-1} + 2A (n-2) 2^{n-2} + 2^n\n",
    "\\]\n",
    "Multiply through by \\(2^{-n+2}\\) (to clear powers):\n",
    "\\[\n",
    "A n \\cdot 4 = A (n-1) \\cdot 2 + 2A (n-2) \\cdot 1 + 4\n",
    "\\]\n",
    "\\[\n",
    "4An = 2A(n-1) + 2A(n-2) + 4\n",
    "\\]\n",
    "\\[\n",
    "4An = 2An - 2A + 2An - 4A + 4\n",
    "\\]\n",
    "\\[\n",
    "4An = 4An - 6A + 4\n",
    "\\]\n",
    "\\[\n",
    "0 = -6A + 4 \\quad \\Rightarrow \\quad A = \\frac{2}{3}\n",
    "\\]\n",
    "So \\(T^{(p)}(n) = \\frac{2}{3} n 2^n\\)\n",
    "\n",
    "**Step 3:** Combine:\n",
    "\\[\n",
    "T(n) = C_1 2^n + C_2 (-1)^n + \\frac{2}{3} n 2^n\n",
    "\\]\n",
    "Use initial:\n",
    "- \\(T(0)=0\\): \\(C_1 + C_2 = 0\\)\n",
    "- \\(T(1)=1\\): \\(2C_1 - C_2 + \\frac{4}{3} = 1\\)\n",
    "Solve: \\(C_1 = -\\frac{1}{9}, C_2 = \\frac{1}{9}\\)\n",
    "\n",
    "\\[\n",
    "\\boxed{T(n) = -\\frac{1}{9} 2^n + \\frac{1}{9} (-1)^n + \\frac{2}{3} n 2^n}\n",
    "\\]\n",
    "\n",
    "---\n",
    "\n",
    "## **Example 4: Merge Sort Complexity**\n",
    "\\[\n",
    "T(n) = 2T\\left(\\frac{n}{2}\\right) + n, \\quad T(1)=1\n",
    "\\]\n",
    "(This is a **divide-by-constant** type, not subtract-by-constant, but shows real CS application)\n",
    "\n",
    "Assume \\(n=2^k\\), let \\(m=k\\):\n",
    "\\[\n",
    "T(2^m) = 2T(2^{m-1}) + 2^m\n",
    "\\]\n",
    "Let \\(S(m) = T(2^m)\\):\n",
    "\\[\n",
    "S(m) = 2S(m-1) + 2^m\n",
    "\\]\n",
    "Homogeneous: \\(S^{(h)}(m) = C \\cdot 2^m\\)\n",
    "Particular: Guess \\(S^{(p)}(m) = A m 2^m\\) (since 2 is a root)\n",
    "Solve: \\(A = 1\\)\n",
    "So \\(S(m) = C 2^m + m 2^m = 2^m(C + m)\\)\n",
    "Since \\(S(0)=T(1)=1\\): \\(1 = 1(C+0)\\) ⇒ \\(C=1\\)\n",
    "\\[\n",
    "S(m) = 2^m(1+m) \\quad \\Rightarrow \\quad T(n) = n(1 + \\log_2 n)\n",
    "\\]\n",
    "\\[\n",
    "\\boxed{T(n) = O(n \\log n)}\n",
    "\\]\n",
    "\n",
    "---\n",
    "\n",
    "## **Common Pitfalls & Tips:**\n",
    "\n",
    "1. **Check if f(n) term matches a root** → multiply by n\n",
    "2. **Always verify with small n values** (n=0,1,2)\n",
    "3. **For divide-by-constant** (like Merge Sort): use substitution \\(n=2^k\\)\n",
    "4. **Complex roots** come in conjugate pairs: \\(a \\pm bi = R(\\cos\\theta \\pm i\\sin\\theta)\\)\n",
    "5. **Initial conditions** must match degree: k-th order needs k initial values\n",
    "\n",
    "---\n",
    "\n",
    "## **When Will You Use This?**\n",
    "\n",
    "- **Exam question:** \"Solve this recurrence\"\n",
    "- **Algorithm design:** Analyzing recursive algorithms\n",
    "- **Dynamic programming:** Closed-form vs recursive solution\n",
    "- **System modeling:** Predicting behavior over time\n",
    "\n",
    "**Remember:** This is just **pattern matching** once you know the forms!"
   ]
  },
  {
   "cell_type": "markdown",
   "id": "801e590a",
   "metadata": {},
   "source": [
    "Excellent question! This is the **most confusing step** for many students. Let me explain **exactly** what we're doing.\n",
    "\n",
    "## **What Does \"Substitute the Guess\" Mean?**\n",
    "\n",
    "When we **guess** a particular solution \\(T^{(p)}(n)\\) based on the form of \\(f(n)\\), we need to **plug it back into the original recurrence equation** to find the unknown coefficients (like \\(A, B, C\\)).\n",
    "\n",
    "---\n",
    "\n",
    "## **Step-by-Step Demonstration:**\n",
    "\n",
    "### **Example:**\n",
    "\\[\n",
    "T(n) = 2T(n-1) + 3T(n-2) + 4n \\quad \\text{(we want to solve this)}\n",
    "\\]\n",
    "\n",
    "---\n",
    "\n",
    "### **Step 1: We've already solved homogeneous part:**\n",
    "Assume we have: \\(T^{(h)}(n) = C_1 r_1^n + C_2 r_2^n\\) (details not needed for this demonstration)\n",
    "\n",
    "---\n",
    "\n",
    "### **Step 2: Guess particular solution:**\n",
    "Since \\(f(n) = 4n\\) is a **polynomial of degree 1**, we guess:\n",
    "\\[\n",
    "T^{(p)}(n) = An + B \\quad \\text{(A and B are unknown constants to find)}\n",
    "\\]\n",
    "\n",
    "---\n",
    "\n",
    "### **Step 3: SUBSTITUTE THIS GUESS INTO ORIGINAL RECURRENCE:**\n",
    "\n",
    "**Original recurrence:** \\(T(n) = 2T(n-1) + 3T(n-2) + 4n\\)\n",
    "\n",
    "**Replace every \\(T(\\cdot)\\) with our guess \\(An+B\\):**\n",
    "\n",
    "Left side: \\(T(n) = An + B\\)\n",
    "\n",
    "Right side:\n",
    "- \\(T(n-1) = A(n-1) + B = An - A + B\\)\n",
    "- \\(T(n-2) = A(n-2) + B = An - 2A + B\\)\n",
    "- So \\(2T(n-1) = 2(An - A + B) = 2An - 2A + 2B\\)\n",
    "- And \\(3T(n-2) = 3(An - 2A + B) = 3An - 6A + 3B\\)\n",
    "- Plus the \\(4n\\) term\n",
    "\n",
    "**Putting right side together:**\n",
    "\\[\n",
    "\\text{Right side} = [2An - 2A + 2B] + [3An - 6A + 3B] + 4n\n",
    "\\]\n",
    "\\[\n",
    "= (2An + 3An + 4n) + (-2A - 6A) + (2B + 3B)\n",
    "\\]\n",
    "\\[\n",
    "= (5A + 4)n + (-8A) + (5B)\n",
    "\\]\n",
    "\n",
    "---\n",
    "\n",
    "### **Step 4: EQUATE LEFT AND RIGHT SIDES:**\n",
    "\n",
    "We have:\n",
    "Left side: \\(An + B\\)\n",
    "Right side: \\((5A + 4)n + (-8A + 5B)\\)\n",
    "\n",
    "These must be **equal for all n**, so coefficients must match:\n",
    "\n",
    "1. **Coefficient of \\(n\\):** \\(A = 5A + 4\\)\n",
    "2. **Constant term:** \\(B = -8A + 5B\\)\n",
    "\n",
    "---\n",
    "\n",
    "### **Step 5: SOLVE THE SYSTEM:**\n",
    "\n",
    "From equation 1: \\(A = 5A + 4 \\Rightarrow -4A = 4 \\Rightarrow A = -1\\)\n",
    "\n",
    "From equation 2: \\(B = -8(-1) + 5B \\Rightarrow B = 8 + 5B \\Rightarrow -4B = 8 \\Rightarrow B = -2\\)\n",
    "\n",
    "---\n",
    "\n",
    "### **Step 6: WRITE PARTICULAR SOLUTION:**\n",
    "\\[\n",
    "T^{(p)}(n) = -n - 2\n",
    "\\]\n",
    "\n",
    "---\n",
    "\n",
    "## **Visual Summary of the Substitution:**\n",
    "\n",
    "```\n",
    "Original:   T(n) = 2T(n-1) + 3T(n-2) + 4n\n",
    "            ↑        ↑          ↑\n",
    "            Replace  Replace    Replace\n",
    "            with     with       with\n",
    "            An+B     A(n-1)+B   A(n-2)+B\n",
    "```\n",
    "\n",
    "We get: \\(An+B = 2[A(n-1)+B] + 3[A(n-2)+B] + 4n\\)\n",
    "\n",
    "---\n",
    "\n",
    "## **Another Example with Exponential:**\n",
    "\n",
    "### **Problem:**\n",
    "\\[\n",
    "T(n) = 3T(n-1) - 2T(n-2) + 5^n\n",
    "\\]\n",
    "\n",
    "**Guess:** \\(T^{(p)}(n) = A \\cdot 5^n\\) (since 5 is not a root)\n",
    "\n",
    "**Substitute:**\n",
    "Left: \\(A \\cdot 5^n\\)\n",
    "Right: \\(3[A \\cdot 5^{n-1}] - 2[A \\cdot 5^{n-2}] + 5^n\\)\n",
    "\n",
    "**Simplify right:** Factor out \\(5^{n-2}\\):\n",
    "\\[\n",
    "5^{n-2}[3A \\cdot 5^1 - 2A \\cdot 5^0] + 5^n = 5^{n-2}[15A - 2A] + 5^n = 13A \\cdot 5^{n-2} + 5^n\n",
    "\\]\n",
    "Better: Write everything with \\(5^n\\):\n",
    "\\[\n",
    "5^n = 3A \\cdot 5^{n-1} - 2A \\cdot 5^{n-2} + 5^n\n",
    "\\]\n",
    "Divide everything by \\(5^{n-2}\\):\n",
    "\\[\n",
    "A \\cdot 5^2 = 3A \\cdot 5^1 - 2A \\cdot 5^0 + 5^2\n",
    "\\]\n",
    "\\[\n",
    "25A = 15A - 2A + 25\n",
    "\\]\n",
    "\\[\n",
    "25A = 13A + 25\n",
    "\\]\n",
    "\\[\n",
    "12A = 25 \\Rightarrow A = \\frac{25}{12}\n",
    "\\]\n",
    "\n",
    "So \\(T^{(p)}(n) = \\frac{25}{12} \\cdot 5^n\\)\n",
    "\n",
    "---\n",
    "\n",
    "## **Why Do We Do This Substitution?**\n",
    "\n",
    "We need to ensure our guess **actually satisfies** the recurrence for the \\(f(n)\\) part. The coefficients \\(A, B, etc.\\) are **adjustment knobs** that make it work.\n",
    "\n",
    "Think of it like this:\n",
    "- **Homogeneous solution:** Satisfies \\(T(n) = aT(n-1) + bT(n-2)\\) with \\(=0\\) on right\n",
    "- **Particular solution:** Must satisfy \\(T(n) = aT(n-1) + bT(n-2) + f(n)\\)\n",
    "- By substituting, we find **exact values** that make the equation true\n",
    "\n",
    "---\n",
    "\n",
    "## **Common Mistakes During Substitution:**\n",
    "\n",
    "1. **Forgetting to adjust for (n-1), (n-2), etc.:**\n",
    "   If \\(T^{(p)}(n) = An + B\\), then:\n",
    "   - \\(T^{(p)}(n-1) = A(n-1) + B\\) NOT \\(An + B\\)\n",
    "   - \\(T^{(p)}(n-2) = A(n-2) + B\\) NOT \\(An + B\\)\n",
    "\n",
    "2. **Not matching coefficients properly:**\n",
    "   After substitution, collect **like terms** (all \\(n\\) terms together, all constants together)\n",
    "\n",
    "3. **Algebra errors with exponents:**\n",
    "   Remember: \\(5^{n-1} = 5^n / 5\\), \\(5^{n-2} = 5^n / 25\\)\n",
    "\n",
    "---\n",
    "\n",
    "## **Quick Check Your Understanding:**\n",
    "\n",
    "For \\(T(n) = T(n-1) + 2T(n-2) + 3\\):\n",
    "Guess: \\(T^{(p)}(n) = A\\) (constant)\n",
    "\n",
    "Substitute:\n",
    "Left: \\(A\\)\n",
    "Right: \\(A + 2A + 3 = 3A + 3\\)\n",
    "\n",
    "Equation: \\(A = 3A + 3 \\Rightarrow -2A = 3 \\Rightarrow A = -\\frac{3}{2}\\)\n",
    "\n",
    "So \\(T^{(p)}(n) = -\\frac{3}{2}\\)\n",
    "\n",
    "**This works!** If \\(T(n) = -\\frac{3}{2}\\) for all n:\n",
    "Left: \\(-\\frac{3}{2}\\)\n",
    "Right: \\((-\\frac{3}{2}) + 2(-\\frac{3}{2}) + 3 = -\\frac{3}{2} - 3 + 3 = -\\frac{3}{2}\\) ✓\n",
    "\n",
    "---\n",
    "\n",
    "## **The Bottom Line:**\n",
    "\n",
    "**Substitution = Plug-and-test** your guess to find the **exact numbers** that make it work. It's like solving a puzzle: \"What values of A, B make this equation true for all n?\"\n",
    "\n",
    "Once you find them, you've got your particular solution!"
   ]
  }
 ],
 "metadata": {
  "kernelspec": {
   "display_name": "Python 3",
   "language": "python",
   "name": "python3"
  },
  "language_info": {
   "name": "python",
   "version": "3.11.9"
  }
 },
 "nbformat": 4,
 "nbformat_minor": 5
}
