{
 "cells": [
  {
   "cell_type": "markdown",
   "id": "a17afc99",
   "metadata": {},
   "source": [
    "## Integral\n",
    "\n",
    "The general rule for integrating $ n^A $ is:\n",
    "\n",
    "$ \\int n^A \\, dn = \\frac{n^{A+1}}{A+1} + C \\quad \\text{(for } A \\ne -1 \\text{)} $\n",
    "\n",
    "$\\text{(for } A = -1 \\text{)} \\int{\\frac{1}{n}} = \\log(n) $\n",
    "\n",
    "---\n",
    "* Integral trick for when it's general form (without $ n^{-1} \\vee (n\\log(n))^{-1} $): \n",
    "    * just multiply by $ n $ \n",
    "\n",
    "$ \\int n^{2}= n^{3} $\n",
    "\n",
    "$ \\int n = n^{2} $\n",
    "\n",
    "$ \\int 1 = \\int n^{0} = n $\n",
    "\n",
    "$ \\int n^{-2}= n^{-1} = \\frac{1}{n} $\n",
    "\n",
    "$ \\int n^{-3}= n^{-2} = \\frac{1}{n^2} $\n",
    "\n",
    "$ \\int n^{-5/2}= \\frac{n^{-5/2 + 1}}{-5/2 + 1} = \\frac{n^{-3/2}}{-3/2} = -\\frac{2}{3} n^{-3/2}  $\n",
    "\n",
    "$ \\int{n^2 \\log(n)} = n^3 \\log(n)$\n",
    "\n",
    "$ \\int{\\frac{n}{\\log(n)}} = \\frac{n^2}{\\log(n)} $\n",
    "\n",
    "$ \\int{\\log(n)} = n\\log(n) $\n",
    "\n",
    "$ \\int{\\frac{1}{\\log(n)}} = n\\frac{1}{\\log(n)} $\n",
    "\n",
    "* Integral trick for when we have $ n^{-1} $ : \n",
    "    * just multiply by $ \\log(n) $\n",
    "\n",
    "    $ \\int{\\frac{1}{n}} = \\log(n) $\n",
    "\n",
    "    $ \\int{\\frac{1}{n} \\log^5(n)} = \\log(n) \\cdot \\log^5(n) = \\log^6(n) $\n",
    "\n",
    "    * (Only to the $ n^{-1} $, other powers don't count as special case for this trick)\n",
    "\n",
    "    $ \\int{\\frac{1}{n^{\\frac{5}{2}}}} = \\int{n^{-\\frac{3}{2}}} =  $\n",
    "\n",
    "* Integral trick for when we have $ (n\\log(n))^{-1} $: \n",
    "    * just multiply by $ \\log(\\log(n)) $ \n",
    "\n",
    "$ \\int{\\frac{1}{n \\log(n)}} = \\log(\\log(n)) $\n",
    "\n",
    "\n",
    "* Use the dominant term (grows slower) Estimation if it's a sum.\n",
    "\n",
    "e.g.\n",
    "\n",
    "$ \\int_1^n \\left( \\frac{1}{n} + \\frac{1}{n^2} \\right) $:\n",
    "\n",
    "$\\int_1^n \\left( \\frac{1}{n} + \\frac{1}{n^2} \\right) =^{DT: \\frac{1}{n}} \\int_1^n ( \\frac{1}{n}) = \\log n \\cdot \\frac{1}{n} = \\frac{\\log n}{n} $\n",
    "\n",
    "---\n",
    "---\n"
   ]
  },
  {
   "cell_type": "markdown",
   "id": "6058d35c",
   "metadata": {},
   "source": [
    "$ T(n) = A \\cdot T(n-1) + f(n) $\n",
    "\n",
    "$ A $ : Shape of the Tree (divisions)\n",
    "\n",
    "$ T(n-1) $ : Height of the Tree\n",
    "\n",
    "$ f(n) $ : Value of nodes\n",
    "\n",
    "$ T(n) $ : Sum of all nodes in all levels\n",
    "\n",
    "---\n",
    "\n",
    "If the nodes at each level sums to $ f(n) $: \n",
    "\n",
    "$ T(n) = L \\cdot f(n) $\n",
    "\n",
    "$ L = 1 + h $\n",
    "\n",
    "\n",
    "e.g.\n",
    "\n",
    "$ T(n) = 4 \\cdot T(\\frac{n}{2}) + n^2 $\n",
    "\n",
    "$ T(n) = (1 + \\log(n))n^2 $\n",
    "\n",
    "not for:\n",
    "\n",
    "$ T(n) = 3 \\cdot T(\\frac{n}{2}) + n^2 $\n",
    "\n",
    "$ T(n) = n^2 \\cdot (1 + \\frac{3}{4} + \\frac{9}{16} + \\dots) = n^2 \\cdot (4 \\vee c) = \\Theta(n^2) $\n",
    "\n",
    "---\n",
    "\n",
    "$ T(n) = A \\cdot T(n-1) + f(n) $ \n",
    "\n",
    "$h = n ,\\quad L = 1 + h = n + 1 $\n",
    "\n",
    "$ T(n) = \\sum_{k=1}^n A^{n-k} f(k) $\n",
    "\n",
    "---\n",
    "$ T(n) = A \\cdot T(n-c) + f(n) $ \n",
    "\n",
    "$h = \\frac{n}{c} ,\\quad L = 1 + h = \\frac{n}{c} + 1 $\n",
    "\n",
    "$ T(n) = \\sum_{k=0}^{\\frac{n}{c}} A^{n-ck} f(ck) $\n",
    "\n",
    "---\n",
    "for $ A \\in \\mathbb{R^+} $\n",
    "\n",
    "$ T(n) = A \\cdot T(\\frac{n}{b}) + f(n) $\n",
    "\n",
    "$ p = \\log_{b}A $\n",
    "\n",
    "$ T(n)= \\Theta(n^p(1 + \\int{\\frac{f(x)}{n^{p+1}}dx} )) $ \n",
    "\n",
    "* Note: the $ T(n) $ could not be less than $ n^p $ regrardless of any $ f(n) $\n",
    "\n",
    "####### e.g.\n",
    "\n",
    "$ T(n) = 2 \\cdot T(\\frac{n}{2}) + \\frac{n}{\\log(n)} $\n",
    "\n",
    "$ p=\\log_{2}2 = 1 $\n",
    "\n",
    "$ T(n)= \\Theta(n^1(1 + \\int{\\frac{\\frac{n}{\\log(n)}}{n^{2}}})) $\n",
    "\n",
    "$ \\int{\\frac{1}{n\\log(n)}} = \\log(\\log(n))$\n",
    "\n",
    "$ T(n)= \\Theta(n + n \\log(\\log(n))) = \\Theta(n \\log(\\log(n))) $\n",
    "\n",
    "####### e.g.\n",
    "\n",
    "$ T(n) = 4 \\cdot T(\\frac{\\sqrt(n)}{4}) + \\log^2(n) $\n",
    "\n",
    "$ n = 2^k \\to k = \\log(n) $\n",
    "\n",
    "$ T(2^k) = 4 \\cdot T(\\frac{\\sqrt(2^k)}{4}) + \\log^2(2^k) = 4 \\cdot T(2^{\\frac{k}{2}}-2) + k^2 = 4 \\cdot T(2^{\\frac{k}{2}}) + k^2 $\n",
    "\n",
    "$ T(2^k) = F(k) \\to F(k) = 4 \\cdot F(\\frac{k}{2}) + k^2$\n",
    "\n",
    "$ p = \\log_2(4) = 2 \\Rightarrow^{\\text{master's}} k^2 \\leq k^2 \\Rightarrow F(k) = \\Theta(k^2 \\cdot \\log(k)) $ \n",
    "\n",
    "$ k = \\log(n) \\to T(n) = \\Theta(\\log^{2}(n) \\cdot \\log(\\log(n))) $\n",
    "\n",
    "---\n",
    "\n",
    "for $ A \\notin \\mathbb{R^+} $\n",
    "\n",
    "$ T(n) = A \\cdot T(\\frac{n}{b}) + f(n) $\n",
    "\n",
    "* we have to devide both sides to make a recursive form out of $ T(n) $ & $ T(n-1) $\n",
    "\n",
    "####### e.g.\n",
    "\n",
    "$ T(n) = n \\cdot T(n-1) + (n+1)! $\n",
    "\n",
    "devide by $ \\quad n! $ : $\\quad \\frac{T(n)}{n!} = \\frac{T(n-1)}{(n-1)!} + (n+1)$  \n",
    "\n",
    "$ F(n)=\\frac{T(n)}{n!} \\rightarrow F(n) = F(n-1) + (n+1) $\n",
    "\n",
    "$ F(n) = \\sum_{i=0}^n (n+1) = \\Theta(n^2) \\rightarrow T(n) = \\Theta(n^2 \\cdot n!) $\n",
    "\n",
    "####### e.g.\n",
    "\n",
    "$ T(n) = \\sqrt{n} \\cdot T(\\sqrt{n}) + n $\n",
    "\n",
    "devide by $ \\quad n $ : $\\quad \\frac{T(n)}{n} = \\frac{T(\\sqrt{n})}{\\sqrt{n}} + 1$  \n",
    "\n",
    "$ F(n)=\\frac{T(\\sqrt{n})}{\\sqrt{n}} \\rightarrow F(n) = F(\\sqrt{n}) + 1 $\n",
    "\n",
    "$ F(n) = \\Theta(\\log(\\log(n))) \\rightarrow T(n) = \\Theta(n \\log(\\log(n))) $\n",
    "\n",
    "\n",
    "\n",
    "---\n",
    "\n",
    "$ T(n) = A \\cdot T(\\log(n)) + f(n) $\n",
    "\n",
    "$ \\begin{cases} T(n) = \\Theta(h) = \\Theta(\\log*(n)) & f(n)=\\Theta(c) \\\\ T(n)=\\Theta(n^{k}) & f(n)=\\Theta(n^{k > 0})\\end{cases} $\n",
    "\n",
    "---\n",
    "\n",
    "General Form of Akra-Bazzi\n",
    "\n",
    "$ T(n) = a_1 T(b_{1}n) + a_2 T(b_{2}n) + f(n) $\n",
    "\n",
    "we have to find $P$ such that:\n",
    "\n",
    "$ \\sum a_i b_i^p = 1 \\to  a_1 b_1^p + a_2 b_2^p = 1 $\n",
    "\n",
    "* if $ \\sum a_i = 1 \\to p=0$\n",
    "* if $ \\sum a_i b_i = 1 \\to p=1$\n",
    "* if for a test p: $ \\sum a_i b_i^p < 1 \\to \\text{lower the} \\quad p $\n",
    "* if for a test p: $ \\sum a_i b_i^p > 1 \\to \\text{increase the} \\quad p $\n",
    "\n",
    "Then:\n",
    "\n",
    "$ T(n)= \\Theta(n^p(1 + \\int{\\frac{f(x)}{n^{p+1}}dx} )) $ \n",
    "\n",
    "\n",
    "* Special case for Akra if $ f(n) = \\theta(n^k) $\n",
    "\n",
    "we try $ p = k \\rightarrow \\begin{cases} T(n) = \\Theta(n^k \\log(n)) & \\sum a_i b_i^p = 1 \\\\ T(n) = \\Theta(n^k) & \\sum a_i b_i^p < 1\\end{cases} $ \n",
    "\n",
    "---\n",
    "\n",
    "$ T(n,k) = T(\\frac{n}{2}, k) + T(n, \\frac{k}{4}) + nk \\quad, T(1,k)=1, \\quad T(n,1)=1$\n",
    "\n",
    "* Backtracking: \n",
    "\n",
    "$ T(n,k) = nk + \\frac{3}{4}nk + \\frac{9}{16}nk + \\frac{27}{64}nk + \\dots $\n",
    "\n",
    "$ T(n,k) = nk (\\frac{1}{1-\\frac{3}{4}}) = 4nk \\rightarrow \\Theta(nk) $\n",
    "\n",
    "\n",
    "---\n",
    "\n",
    "Time Complexity of F: \n",
    "\n",
    "how many times the F calls for itself = the count of nodes in the recursion tree.\n",
    "\n",
    "---\n",
    "Time complexity for :\n",
    "\n",
    "$$\n",
    "F(n, m) = \n",
    "\\begin{cases}\n",
    "1 & \\text{if } n \\leq 1 \\parallel m \\leq 1 \\\\\n",
    "n + m \\cdot F(n-1, \\frac{m}{2}) & \\text{otherwise}\n",
    "\\end{cases}\n",
    "$$\n",
    "\n",
    "* for $ \\parallel $ :$ \\text{Time Complexity} = 1 + \\min \\begin{cases} h_n = n \\\\ h_m=\\log_2(m) \\end{cases} $\n",
    "\n",
    "* for && :$ \\text{Time Complexity} = 1 + \\max \\begin{cases} h_n = n \\\\ h_m=\\log_2(m) \\end{cases} $"
   ]
  },
  {
   "cell_type": "markdown",
   "id": "325f6971",
   "metadata": {},
   "source": [
    "Linear RRs\n",
    "\n",
    "Standard Form: <br/>$T(n) = a_1T(n-1) + a_2T(n-2) + \\cdots + a_kT(n-k) + f(n) $ \n",
    "\n",
    "Homogeneous part:<br/> $T(n) = a_1T(n-1) + a_2T(n-2) + \\cdots + a_kT(n-k) $ \n",
    "\n",
    "none-Homogeneous part (Particular solution):<br/> $f(n) $ \n",
    "\n",
    "---\n",
    "### Step 1: Solve the characteristic equation for Homogeneous Part\n",
    "\n",
    "$ T(n) - a_1T(n-1) - a_2T(n-2) - \\cdots - a_kT(n-k) = 0 $ <br/>\n",
    "$ T(n) = r^n \\rightarrow r^n = a_1 r^{n-1} + a_2 r^{n-2} + \\cdots + a_k r^{n-k}$ <br/>\n",
    "Divide by $r^{n-k} \\rightarrow r^k = a_1 r^{k-1} + a_2 r^{k-2} + \\cdots + a_k$ <br/>\n",
    "\n",
    "Rewrite as: <br/> $r^k - a_1 r^{k-1} - a_2 r^{k-2} - \\cdots - a_k = 0$\n",
    "* rewrite the smallest as $r^0$ and then increment the power of r by one for bigger ones\n",
    "\n",
    "solve for the $r$ : $ \\begin{cases}\\text{Distinct real roots} & T^{(h)}(n) = C_1 r_1^n + C_2 r_2^n \\\\ \\text{Repeated root r (multiplicity m)} & T^{(h)}(n) = r^n + n r^n\\end{cases} $\n",
    "\n",
    "---\n",
    "### Step 2: guess Particular Solution\n",
    "For $f(n) \\neq 0 $, guess a form similar to $ f(n) = cn^k \\cdot A^n $ in which the $ cn^k $ is complete polynomial with unkown $ c_i $ <br/> \n",
    "\n",
    "$ T^{(p)}(n) = (c_1n^k + c_2n^{k-1} + \\dots + c_n) A^n$\n",
    "\n",
    "###e.g. <br/>\n",
    "for $ f(n)=3n5^n \\to cn^k \\cdot A^n = 3n^1 \\cdot 5^n \\to T^{(p)}(n) = (c_1n^1 + c_2) 5^n$ <br/>\n",
    "for $ f(n)=6n^2 \\to cn^k \\cdot A^n = 6n^2 \\cdot 0^n \\to T^{(p)}(n) = (c_1n^2 + c_2n^1 + c_3) 0^n$\n",
    "\n",
    "Substitute guess into original recurrence to solve for the unknown coefficients.  rewrite $T(n)$ as $T^{(p)}(n) $ and do keep in mind that you want to formulate the equation to look like $T^{(p)}(n)$ after substituiton.\n",
    "\n",
    "###e.g. <br/>\n",
    "$ T(n) = 2T(n-1) + 3T(n-2) + 4n$ <br/>\n",
    "$ T^{(p)}(n) = c_1 n + c_2$ <br/>\n",
    "substitution: $ c_1 n + c_2 = 2(c_1 (n-1) + c_2) + 3(c_1 (n-2) + c_2) = (5c_1 + 4)n + (-8c_1) + (5c_2)$ <br/>\n",
    "$ \\to  c_1 n + c_2 = (5c_1 + 4)n + (-8c_1) + (5c_2)$\n",
    "\n",
    "for all n: $ \\begin{cases} c_1 = 5c_1 + 4 \\\\ c_2 = (-8c_1) + (5c_2) \\end{cases} \\Rightarrow  \\begin{cases} c_1 = -1 \\\\ c_2 = -2 \\end{cases} \\Rightarrow T^{(p)}(n) = -1 n -2$\n",
    "\n",
    "\n",
    "\n",
    "---\n",
    "\n",
    "### Step 3: Combine and Solve for Constants\n",
    "\n",
    "* if there is similar expression in both $T^{(h)}(n)$ and $T^{(p)}(n)$, we have to multiply the one in $T^{(p)}(n)$ by $n$\n",
    "\n",
    "\n",
    "$T(n) = T^{(h)}(n) + T^{(p)}(n)$\n",
    "\n",
    "Use initial conditions (like $ T(0), T(1), \\ldots $) to find $ C_1, C_2, \\ldots$"
   ]
  },
  {
   "cell_type": "markdown",
   "id": "afe8110e",
   "metadata": {},
   "source": [
    "# **Tower of Hanoi: Two Forms with Recurrence Solutions**\n",
    "\n",
    "## **Form 1: Classic Tower of Hanoi**\n",
    "\n",
    "### **Problem Statement:**\n",
    "- 3 pegs: A (source), B (auxiliary), C (destination)\n",
    "- n disks of different sizes on peg A\n",
    "- Can only move one disk at a time\n",
    "- Never place larger disk on smaller disk\n",
    "- Goal: Move all disks from A to C\n",
    "\n",
    "---\n",
    "\n",
    "### **Recurrence Relation:**\n",
    "Let \\(T_1(n)\\) = minimum moves for n disks in classic Hanoi\n",
    "\n",
    "**Reasoning:**\n",
    "1. Move (n-1) disks from A to B (using C as auxiliary): \\(T_1(n-1)\\) moves\n",
    "2. Move largest disk from A to C: 1 move\n",
    "3. Move (n-1) disks from B to C (using A as auxiliary): \\(T_1(n-1)\\) moves\n",
    "\n",
    "\\[\n",
    "T_1(n) = 2T_1(n-1) + 1, \\quad T_1(1) = 1\n",
    "\\]\n",
    "\n",
    "---\n",
    "\n",
    "### **Solving the Recurrence:**\n",
    "\n",
    "**Step 1: Homogeneous part:**\n",
    "\\[\n",
    "T_1(n) - 2T_1(n-1) = 0\n",
    "\\]\n",
    "Characteristic: \\(r - 2 = 0 \\Rightarrow r = 2\\)\n",
    "\\[\n",
    "T_1^{(h)}(n) = C \\cdot 2^n\n",
    "\\]\n",
    "\n",
    "**Step 2: Particular solution:**\n",
    "\\(f(n) = 1\\) (constant)\n",
    "Guess: \\(T_1^{(p)}(n) = A\\) (constant)\n",
    "\n",
    "Substitute: \\(A = 2A + 1 \\Rightarrow -A = 1 \\Rightarrow A = -1\\)\n",
    "So \\(T_1^{(p)}(n) = -1\\)\n",
    "\n",
    "**Step 3: General solution:**\n",
    "\\[\n",
    "T_1(n) = C \\cdot 2^n - 1\n",
    "\\]\n",
    "\n",
    "**Step 4: Apply initial condition:**\n",
    "\\(T_1(1) = 1\\):\n",
    "\\[\n",
    "C \\cdot 2^1 - 1 = 1 \\Rightarrow 2C - 1 = 1 \\Rightarrow 2C = 2 \\Rightarrow C = 1\n",
    "\\]\n",
    "\n",
    "\\[\n",
    "\\boxed{T_1(n) = 2^n - 1}\n",
    "\\]\n",
    "\n",
    "**Verification:** \n",
    "- \\(n=1\\): \\(2^1 - 1 = 1\\) ✓\n",
    "- \\(n=2\\): \\(2^2 - 1 = 3\\) ✓ (AB, AC, BC)\n",
    "- \\(n=3\\): \\(2^3 - 1 = 7\\) ✓\n",
    "\n",
    "---\n",
    "\n",
    "## **Form 2: Restricted Tower of Hanoi (A→C moves only allowed)**\n",
    "\n",
    "### **Problem Statement (Reve's Puzzle variant):**\n",
    "- Same 3 pegs A, B, C\n",
    "- Same n disks\n",
    "- **Restriction:** Direct moves from A→C and C→A are **NOT ALLOWED**\n",
    "- Must always go through B\n",
    "- Still can't place larger on smaller\n",
    "\n",
    "This is sometimes called the \"Cyclic Hanoi\" or \"Reve's Puzzle\" with restriction.\n",
    "\n",
    "---\n",
    "\n",
    "### **Recurrence Relation:**\n",
    "Let \\(T_2(n)\\) = minimum moves for n disks with A→C restriction\n",
    "\n",
    "**To move n disks from A to C:**\n",
    "1. Move (n-1) disks from A to C (but wait, A→C direct not allowed! Need different strategy...)\n",
    "\n",
    "Actually, with A→C restriction:\n",
    "**Strategy:**\n",
    "1. Move (n-1) disks from A to B (using C): \\(T_2(n-1)\\) moves\n",
    "2. Move largest disk from A to B: 1 move (A→B allowed)\n",
    "3. Move (n-1) disks from B to C (using A): \\(T_2(n-1)\\) moves\n",
    "4. Move largest disk from B to C: 1 move (B→C allowed)\n",
    "\n",
    "But wait, steps 2 and 4 require moving largest disk twice! Actually...\n",
    "\n",
    "**Correct reasoning:**\n",
    "To move n disks from A to C with no A→C moves:\n",
    "1. Move (n-1) disks from A to C: \\(T_2(n-1)\\) moves\n",
    "   (But this requires moving them through B since A→C not allowed)\n",
    "   \n",
    "Actually, let's think systematically:\n",
    "\n",
    "Let's define:\n",
    "- \\(T_2(n)\\) = moves to transfer n disks from A to C with restriction\n",
    "\n",
    "**To move n disks from A to C:**\n",
    "1. Move (n-1) disks from A to B (using C): \\(T_2(n-1)\\) moves\n",
    "   (But to move from A to B, that's allowed, no restriction issue)\n",
    "2. Move largest disk from A to C: **NOT ALLOWED!** So can't do this.\n",
    "\n",
    "We need a **different approach**. With A→C restriction:\n",
    "\n",
    "**Actually, here's the correct recurrence:**\n",
    "We need to move n disks from A to C without direct A→C moves.\n",
    "\n",
    "One valid strategy:\n",
    "1. Move (n-1) disks from A to C (but through B somehow): Let's call this \\(T_2(n-1)\\)\n",
    "   Actually, to move from A to C without direct moves, we need to go A→B→C\n",
    "   \n",
    "Better: Define \\(T_2(n)\\) = moves to move n disks from A to C with restriction\n",
    "\n",
    "**Think recursively:**\n",
    "To move n disks A→C without A→C moves:\n",
    "1. Move (n-1) disks from A to C: Can't be \\(T_2(n-1)\\) because that's what we're trying to compute!\n",
    "\n",
    "Actually, the known recurrence for this restricted version (Reve's Puzzle with A↔C forbidden) is:\n",
    "\\[\n",
    "T_2(n) = 3T_2(n-1) + 2\n",
    "\\]\n",
    "With \\(T_2(1) = 2\\) (A→B→C)\n",
    "\n",
    "---\n",
    "\n",
    "### **Why \\(T_2(n) = 3T_2(n-1) + 2\\)?**\n",
    "\n",
    "**Reasoning:**\n",
    "To move n disks from A to C (no A→C):\n",
    "1. Move (n-1) disks from A to C: \\(T_2(n-1)\\) moves\n",
    "   Wait, that doesn't make sense... We need to think differently.\n",
    "\n",
    "Actually, the known strategy:\n",
    "1. Move (n-1) disks from A to B (using C): \\(T_2(n-1)\\) moves\n",
    "2. Move largest disk from A to C: **NOT ALLOWED!**\n",
    "   So instead: Move largest disk A→B (1 move)\n",
    "3. Move (n-1) disks from B to C: \\(T_2(n-1)\\) moves\n",
    "4. Move largest disk from B to C: 1 move\n",
    "\n",
    "That gives: \\(T_2(n) = 2T_2(n-1) + 2\\)\n",
    "\n",
    "But actually, step 3 \"Move (n-1) disks from B to C\" might not be \\(T_2(n-1)\\) because that's defined for A→C moves.\n",
    "\n",
    "The correct known recurrence for \"no direct moves between source and destination\" is actually:\n",
    "\\[\n",
    "T_2(n) = 3T_2(n-1) + 2\n",
    "\\]\n",
    "Because:\n",
    "1. Move (n-1) disks from A to B: \\(T_2(n-1)\\)\n",
    "2. Move largest disk A→B: 1\n",
    "3. Move (n-1) disks from B to C: \\(T_2(n-1)\\)\n",
    "4. Move largest disk B→C: 1\n",
    "5. But wait, we still have (n-1) disks on C that need to go... Actually, this is getting messy.\n",
    "\n",
    "Let me give you the **actual standard solution** for restricted Hanoi:\n",
    "\n",
    "---\n",
    "\n",
    "### **Known Standard Solution:**\n",
    "\n",
    "For Tower of Hanoi with **A→C moves forbidden** (must go A→B→C):\n",
    "\\[\n",
    "T_2(n) = 3T_2(n-1) + 2, \\quad T_2(1) = 2\n",
    "\\]\n",
    "\n",
    "**Reason:** To move n disks from A to C:\n",
    "1. Move (n-1) disks from A to C: \\(T_2(n-1)\\) moves\n",
    "   (Yes, this is possible by going A→B→C for each disk recursively)\n",
    "2. Move largest disk from A to B: 1 move\n",
    "3. Move (n-1) disks from C to A: \\(T_2(n-1)\\) moves\n",
    "4. Move largest disk from B to C: 1 move\n",
    "5. Move (n-1) disks from A to C: \\(T_2(n-1)\\) moves\n",
    "\n",
    "Total: \\(3T_2(n-1) + 2\\)\n",
    "\n",
    "---\n",
    "\n",
    "### **Solving \\(T_2(n) = 3T_2(n-1) + 2\\):**\n",
    "\n",
    "**Step 1: Homogeneous:**\n",
    "\\[\n",
    "T_2(n) - 3T_2(n-1) = 0\n",
    "\\]\n",
    "Characteristic: \\(r - 3 = 0 \\Rightarrow r = 3\\)\n",
    "\\[\n",
    "T_2^{(h)}(n) = C \\cdot 3^n\n",
    "\\]\n",
    "\n",
    "**Step 2: Particular:**\n",
    "\\(f(n) = 2\\) (constant)\n",
    "Guess: \\(T_2^{(p)}(n) = A\\)\n",
    "\n",
    "Substitute: \\(A = 3A + 2 \\Rightarrow -2A = 2 \\Rightarrow A = -1\\)\n",
    "So \\(T_2^{(p)}(n) = -1\\)\n",
    "\n",
    "**Step 3: General solution:**\n",
    "\\[\n",
    "T_2(n) = C \\cdot 3^n - 1\n",
    "\\]\n",
    "\n",
    "**Step 4: Apply initial:**\n",
    "\\(T_2(1) = 2\\):\n",
    "\\[\n",
    "C \\cdot 3^1 - 1 = 2 \\Rightarrow 3C - 1 = 2 \\Rightarrow 3C = 3 \\Rightarrow C = 1\n",
    "\\]\n",
    "\n",
    "\\[\n",
    "\\boxed{T_2(n) = 3^n - 1}\n",
    "\\]\n",
    "\n",
    "**Verification:**\n",
    "- \\(n=1\\): \\(3^1 - 1 = 2\\) ✓ (A→B, B→C)\n",
    "- \\(n=2\\): \\(3^2 - 1 = 8\\) ✓\n",
    "- \\(n=3\\): \\(3^3 - 1 = 26\\) ✓\n",
    "\n",
    "---\n",
    "\n",
    "## **Comparison Summary:**\n",
    "\n",
    "| Aspect | Classic Hanoi | Restricted Hanoi (No A→C) |\n",
    "|--------|--------------|--------------------------|\n",
    "| **Recurrence** | \\(T_1(n) = 2T_1(n-1) + 1\\) | \\(T_2(n) = 3T_2(n-1) + 2\\) |\n",
    "| **Initial** | \\(T_1(1) = 1\\) | \\(T_2(1) = 2\\) |\n",
    "| **Solution** | \\(T_1(n) = 2^n - 1\\) | \\(T_2(n) = 3^n - 1\\) |\n",
    "| **Growth** | Exponential base 2 | Exponential base 3 |\n",
    "| **For n=3** | 7 moves | 26 moves |\n",
    "| **For n=5** | 31 moves | 242 moves |\n",
    "\n",
    "---\n",
    "\n",
    "## **Interesting Observations:**\n",
    "\n",
    "1. **The restriction makes it MUCH harder:** \\(3^n - 1\\) grows much faster than \\(2^n - 1\\)\n",
    "   \n",
    "2. **Ratio:** \\(\\frac{T_2(n)}{T_1(n)} \\approx \\left(\\frac{3}{2}\\right)^n\\) for large n\n",
    "\n",
    "3. **Both follow the same solution pattern:**\n",
    "   - Guess particular solution as constant\n",
    "   - Get homogeneous solution as \\(C \\cdot r^n\\)\n",
    "   - Combine and use initial condition\n",
    "\n",
    "4. **The method works perfectly** for both, even though the constants and coefficients differ.\n",
    "\n",
    "---\n",
    "\n",
    "## **Why Both Are Solvable with Our Method:**\n",
    "\n",
    "Both recurrences are of the form:\n",
    "\\[\n",
    "T(n) = aT(n-1) + b\n",
    "\\]\n",
    "Where:\n",
    "- Classic: \\(a=2, b=1\\)\n",
    "- Restricted: \\(a=3, b=2\\)\n",
    "\n",
    "General solution for \\(T(n) = aT(n-1) + b\\):\n",
    "1. Homogeneous: \\(T^{(h)}(n) = C \\cdot a^n\\)\n",
    "2. Particular: Guess \\(A\\), get \\(A = aA + b \\Rightarrow A = \\frac{b}{1-a}\\) (if \\(a \\neq 1\\))\n",
    "3. \\(T(n) = C a^n + \\frac{b}{1-a}\\)\n",
    "4. Use \\(T(1)\\) to find C\n",
    "\n",
    "For classic: \\(A = \\frac{1}{1-2} = -1\\), so \\(T_1(n) = C \\cdot 2^n - 1\\)\n",
    "For restricted: \\(A = \\frac{2}{1-3} = -1\\), so \\(T_2(n) = C \\cdot 3^n - 1\\)\n",
    "\n",
    "**Same pattern, different constants!**"
   ]
  }
 ],
 "metadata": {
  "kernelspec": {
   "display_name": "Python 3",
   "language": "python",
   "name": "python3"
  },
  "language_info": {
   "name": "python",
   "version": "3.11.9"
  }
 },
 "nbformat": 4,
 "nbformat_minor": 5
}
